Add files via upload

SmallSteps.thy
@@ -22,11 +22,14 @@ section "The fine-grained (small) computation steps"
 type_synonym 's config = "'s LA \<times> 's"
 
 
-abbreviation stateOf :: "'s config \<times> bool \<Rightarrow> 's"
-  where "stateOf cf \<equiv> snd(fst cf)"
+abbreviation confOf :: "'s config \<times> bool \<Rightarrow> 's config"
+  where "confOf cf \<equiv> fst(cf)"
 
 abbreviation progOf :: "'s config \<times> bool \<Rightarrow> 's LA"
-  where "progOf cf \<equiv> fst(fst cf)"
+  where "progOf cf \<equiv> fst(confOf cf)"
+
+abbreviation stateOf :: "'s config \<times> bool \<Rightarrow> 's"
+  where "stateOf cf \<equiv> snd(confOf cf)"
 
 abbreviation tkOf :: "'s config \<times> bool \<Rightarrow> bool"
   where "tkOf cf \<equiv> snd(cf)"
@@ -105,8 +108,7 @@ lemma pstep_Jump :
 
 
 lemma jumpfree_pstep' :
-"\<rho> \<turnstile> cf -p\<rightarrow> cf' \<Longrightarrow>
- jumpfree (fst cf) \<Longrightarrow>
+"\<rho> \<turnstile> cf -p\<rightarrow> cf' \<Longrightarrow> jumpfree (fst cf) \<Longrightarrow>
  jumpfree (fst cf')"
   apply(induct cf cf' rule: pstep.induct, simp_all)
   apply clarsimp
@@ -121,10 +123,20 @@ lemma jumpfree_pstep' :
   done
 
 corollary jumpfree_pstep :
-"\<rho> \<turnstile> (p, s) -p\<rightarrow> (q, t) \<Longrightarrow>
- jumpfree p \<Longrightarrow>
+"\<rho> \<turnstile> (p, s) -p\<rightarrow> (q, t) \<Longrightarrow> jumpfree p \<Longrightarrow>
  jumpfree q"
   by(drule jumpfree_pstep', simp_all)
+
+
+lemma jumpfree_locally_seq_pstep' :
+"\<rho> \<turnstile> cf -p\<rightarrow> cf' \<Longrightarrow> jumpfree (fst cf) \<Longrightarrow> locally_seq (fst cf) \<Longrightarrow>
+ locally_seq (fst cf')"
+  by(induct cf cf' rule: pstep.induct, simp_all)
+
+corollary jumpfree_locally_seq_pstep :
+"\<rho> \<turnstile> (p, s) -p\<rightarrow> (q, t) \<Longrightarrow> jumpfree p \<Longrightarrow> locally_seq p \<Longrightarrow>
+ locally_seq q"
+  by(drule jumpfree_locally_seq_pstep', simp_all)
 
 
 
@@ -218,6 +230,78 @@ lemma Await_pstep :
  s \<in> C \<and> \<rho> \<turnstile> (p, s) -p\<rightarrow>\<^sup>* (SKIP, t) \<and> p' = SKIP"
   by(erule pstep.cases, simp_all)
 
+
+lemma locally_seq_jumpfree_pstep_unq_aux :
+"(\<lambda>x1 x2. \<rho> \<turnstile> x1 -p\<rightarrow> x2 \<and> (\<forall>a b. \<rho> \<turnstile> x1 -p\<rightarrow> (a, b) \<longrightarrow> locally_seq (fst x1) \<longrightarrow> jumpfree (fst x1) \<longrightarrow> x2 = (a, b)))\<^sup>*\<^sup>* cf cf' \<Longrightarrow>
+ \<rho> \<turnstile> cf -p\<rightarrow>\<^sup>* cf'' \<Longrightarrow> 
+ locally_seq (fst cf) \<Longrightarrow>
+ jumpfree (fst cf) \<Longrightarrow>
+ fst cf' = Skip \<Longrightarrow>
+ fst cf'' = Skip \<Longrightarrow>
+ cf' = cf''"
+  apply(induct cf arbitrary: cf'' rule: converse_rtranclp_induct)
+   apply(case_tac cf', clarsimp)
+   apply(subst (asm) rtranclp_power)
+   apply clarify
+   apply(case_tac n, clarsimp)
+   apply clarify
+   apply(erule relpowp_Suc_E2)
+   apply(clarsimp, erule Skip_pstep)
+  apply clarify
+  apply(rename_tac p1 s1 p2 s2 p3 s3)
+  apply(drule_tac x=p3 in meta_spec)
+  apply(drule_tac x=s3 in meta_spec)
+  apply(drule meta_mp)
+   apply(subst (asm) rtranclp_power)+
+   apply clarify
+   apply(rename_tac m)
+   apply(case_tac m)
+    apply(thin_tac "\<forall>a. _ a")
+    apply clarsimp
+    apply(erule Skip_pstep)
+   apply clarify
+   apply(rename_tac m')
+   apply(erule relpowp_Suc_E2, clarify)
+   apply(rename_tac p s)
+   apply(drule_tac x=p in spec, drule_tac x=s in spec)
+   apply clarsimp
+   apply(subst rtranclp_power, fast)
+  apply(thin_tac "\<forall>a. _ a")
+  apply(drule meta_mp, simp)
+   apply(erule jumpfree_locally_seq_pstep, assumption+)
+  apply(drule meta_mp, simp)
+   apply(erule jumpfree_pstep, assumption)
+  apply simp
+  done
+
+
+
+lemma locally_seq_jumpfree_pstep_unq' :
+"\<rho> \<turnstile> cf -p\<rightarrow> cf' \<Longrightarrow> \<rho> \<turnstile> cf -p\<rightarrow> cf'' \<Longrightarrow> locally_seq (fst cf) \<Longrightarrow> jumpfree (fst cf) \<Longrightarrow>
+ cf' = cf''"
+  apply(induct cf cf' arbitrary: cf'' rule: pstep.induct, simp_all)
+         apply clarsimp
+         apply(drule Basic_pstep, clarsimp)
+        apply(case_tac "p\<^sub>1 = Skip", clarify)
+         apply(erule Skip_pstep)
+        apply clarify
+        apply(drule Seq_pstep, assumption)
+        apply blast
+       apply clarify
+       apply(drule Seq_pstep_Skip, clarsimp+)
+      apply(drule Cond_pstep, clarsimp+)+
+    apply(drule While_pstep, clarsimp+)+
+  apply(drule Await_pstep, clarsimp)
+  apply(drule locally_seq_jumpfree_pstep_unq_aux, assumption)
+  by simp+
+
+
+corollary locally_seq_jumpfree_pstep_unq :
+"\<rho> \<turnstile> (p, s) -p\<rightarrow> (p1, t1) \<Longrightarrow> \<rho> \<turnstile> (p, s) -p\<rightarrow> (p2, t2) \<Longrightarrow> locally_seq p \<Longrightarrow> jumpfree p \<Longrightarrow>
+  p1 = p2 \<and> t1 = t2"
+  apply(drule locally_seq_jumpfree_pstep_unq')
+     apply assumption
+  by simp+
 
 
 end
