Fairness.thy
@@ -1,0 +1,240 @@
+(* *********************************************************************
+
+    Theory Fairness.thy is part of a framework for modelling,
+    verification and transformation of concurrent imperative
+    programs. Copyright (c) 2021  M. Bortin
+
+    The framework is distributed in the hope that it will be useful,
+    but WITHOUT ANY WARRANTY; without even the implied warranty of
+    MERCHANTABILITY or FITNESS FOR A PARTICULAR PURPOSE.
+    For more details see the license agreement (LICENSE) you should have
+    received along with the framework.
+    
+   ******************************************************************* *)
+
+theory Fairness
+imports Positions 
+begin
+
+subsection "Always available program positions"
+
+text "defines positions that are generally available for a reduction so that 
+      the subsequently presented notion of fairness gets comparably weak 
+      as it does not address evaluation of await-statements 
+      except terminating atomic sections"
+definition "available_pos \<rho> p = {xs. xs \<in> set(rpos p) \<and> 
+                                (case p|\<^bsub>xs\<^esub> of
+                                  Some (Await C a p) \<Rightarrow> (C = UNIV \<and> (\<forall>s. \<exists>t. \<rho> \<turnstile> (p, s) -p\<rightarrow>\<^sup>* (Skip, t)))
+                                | _ \<Rightarrow> True)}"
+lemma available_rpos :
+"xs \<in> available_pos \<rho> p \<Longrightarrow> 
+ xs \<in> set(rpos p)"
+  by(simp add: available_pos_def)
+
+
+lemma available_pos_pstep' :
+"xs \<in> available_pos \<rho> p \<Longrightarrow>
+ \<exists>p' t. \<rho> \<turnstile> (the(p|\<^bsub>xs\<^esub>), s) -p\<rightarrow> (p', t)" 
+  apply(clarsimp simp: available_pos_def)
+  apply(induct p xs rule: lookup_pos.induct)
+    apply(drule rpos_noNil, clarify)
+   apply(frule rpos_singleton)
+   apply clarsimp
+   apply(case_tac p, clarsimp+)
+         apply(intro exI, rule pstep.Basic)
+        apply(clarsimp split: if_splits)
+         apply(intro exI, rule pstep.SeqSkip)
+        apply(drule rpos_noNil, clarify)
+       apply clarsimp
+       apply(rename_tac C p q)
+       apply(case_tac "s \<in> C")
+        apply(intro exI, erule pstep.CondT)
+       apply(intro exI, erule pstep.CondF)
+      apply clarsimp
+      apply(rename_tac C I p q)
+      apply(case_tac "s \<in> C")
+       apply(intro exI, erule pstep.WhileT)
+      apply(intro exI, erule pstep.WhileF)
+     apply(clarsimp split: if_splits)
+     apply(intro exI, rule pstep.ParallelSkip, fastforce)
+    apply clarsimp
+    apply(drule_tac x=s in spec, clarify)
+    apply(intro exI, rule pstep.Await, simp+)
+   apply(rename_tac C p q)
+   apply(case_tac "s \<in> C")
+    apply(intro exI, erule CJumpT)
+   apply(intro exI, erule CJumpF)
+  apply(rename_tac x' xs)
+  apply clarsimp
+  apply(rule conjI, clarsimp)
+   apply(case_tac p, simp_all)
+    apply(clarsimp split: if_splits)+
+  apply(case_tac p, simp_all)
+   apply(clarsimp split: if_splits)+
+  done
+
+text "thus, the subterm at an available position always amounts to a program step"
+corollary available_pos_pstep :
+"xs \<in> available_pos \<rho> p \<Longrightarrow>
+ \<exists>p' t. \<rho> \<turnstile> (the(lookup_pos p xs), s) -p\<rightarrow> (p', t) \<and>
+        \<rho> \<turnstile> (p, s) -p\<rightarrow> (p\<lbrakk>p'\<rbrakk>\<^bsub>xs\<^esub>, t)"
+  apply(frule_tac s=s in available_pos_pstep')
+  apply clarify
+  apply(drule available_rpos)
+  apply(drule rpos_pstep, assumption)
+  by fast
+
+
+
+lemma iCOMP_available_pos_retain :
+"sq \<in> iCOMP \<rho> \<Longrightarrow> fair_ret \<rho> \<Longrightarrow> xs\<in>available_pos \<rho> (progOf(sq i)) \<Longrightarrow> i < j \<Longrightarrow>
+ \<forall>k\<ge>i. k < j \<longrightarrow> tkOf(sq(k+1)) \<longrightarrow> (progOf(sq k))|\<^bsub>xs\<^esub> = (progOf(sq i))|\<^bsub>xs\<^esub> \<longrightarrow> 
+        fpos_of \<rho> (confOf(sq k)) (confOf(sq(k+1))) \<noteq> xs \<Longrightarrow>
+ xs\<in>available_pos \<rho> (progOf(sq j)) \<and> (progOf(sq i))|\<^bsub>xs\<^esub> = (progOf(sq j))|\<^bsub>xs\<^esub>"
+  apply(drule_tac xs=xs in iCOMP_rpos_retain, assumption)
+     apply(erule available_rpos)
+    apply assumption+
+  apply(clarsimp simp: available_pos_def)
+  done
+
+
+
+subsection "Fair potential computations"
+
+
+definition
+"fair_iCOMP \<rho> = {sq. sq \<in> iCOMP \<rho> \<and> 
+ (\<forall>i. (\<forall>xs\<in>available_pos \<rho> (progOf(sq i)). 
+  \<exists>j\<ge>i. tkOf(sq(j+1)) \<and> (progOf(sq j))|\<^bsub>xs\<^esub> = (progOf(sq i))|\<^bsub>xs\<^esub> \<and> 
+        fpos_of \<rho> (confOf(sq j)) (confOf(sq(j+1))) = xs))}"
+
+
+lemma fair_iCOMP_D1 :
+"sq \<in> fair_iCOMP \<rho> \<Longrightarrow> sq \<in> iCOMP \<rho>"
+  by(simp add: fair_iCOMP_def)
+
+lemma fair_iCOMP_D2 :
+"sq \<in> fair_iCOMP \<rho> \<Longrightarrow> xs \<in> available_pos \<rho> (progOf(sq i)) \<Longrightarrow> 
+  \<exists>j\<ge>i. tkOf(sq(j+1)) \<and> (progOf(sq j))|\<^bsub>xs\<^esub> = (progOf(sq i))|\<^bsub>xs\<^esub> \<and> 
+        fpos_of \<rho> (confOf(sq j)) (confOf(sq (j+1))) = xs"
+  by(simp add: fair_iCOMP_def)
+
+
+lemma fair_iCOMP_isuffix :
+"sq \<in> fair_iCOMP \<rho> \<Longrightarrow> isuffix sq d \<in> fair_iCOMP \<rho>"
+  apply(clarsimp simp: fair_iCOMP_def)
+  apply(rule conjI)
+   apply(erule iCOMP_isuffix)
+  apply clarsimp
+  apply(drule_tac x="i+d" in spec)
+  apply(clarsimp simp: isuffix_def)
+  apply(drule bspec, assumption)
+  apply clarsimp
+  apply(rule_tac x="j-d" in exI, simp)
+  done
+
+
+lemma isuffix_fair_iCOMP :
+"isuffix sq d \<in> fair_iCOMP \<rho> \<Longrightarrow> sq \<in> iCOMP \<rho> \<Longrightarrow> fair_ret \<rho> \<Longrightarrow> sq \<in> fair_iCOMP \<rho>"
+  apply(subst fair_iCOMP_def, clarsimp)
+  apply(case_tac "i \<ge> d")
+   apply(drule_tac i="i-d" and xs=xs in fair_iCOMP_D2)
+    apply(clarsimp simp: isuffix_def)+
+   apply(rule_tac x="j+d" in exI, simp)
+  apply(rule ccontr)
+  apply(drule_tac i=i and j=d in iCOMP_available_pos_retain)
+      apply assumption+
+    apply fastforce+
+  apply(drule_tac i=0 and xs=xs in fair_iCOMP_D2)
+   apply(clarsimp simp: isuffix_def)
+  apply(drule not_le_imp_less)
+  apply(erule notE)
+  apply clarify
+  apply(rule_tac x="j+d" in exI)
+  apply(clarsimp simp: isuffix_def)
+  done
+
+
+
+subsection "A construction of fair computations"
+
+text "this simple construction just keeps evaluating
+      the given program p in a state s as long as an
+      available position is present and yields to the 
+      'stuttering' environment otherwise, which is fair
+      if there cannot be more than one available position
+      (this is the case with locally sequential jumpfree programs)"
+fun fair_seq where
+"fair_seq \<rho> p s 0 = ((p, s), True)" |
+"fair_seq \<rho> p s (Suc n) = 
+ (let ((p', s'), tk) = fair_seq \<rho> p s n in
+  if \<exists>xs. xs \<in> available_pos \<rho> p' 
+  then (SOME x. \<rho> \<turnstile> (p', s') -p\<rightarrow> x, True)
+  else ((p', s'), False))"
+
+
+
+lemma fair_seq_iCOMP :
+"fair_seq \<rho> p s \<in> iCOMP \<rho>"
+  apply(clarsimp simp: iCOMP_def)
+  apply(case_tac "fair_seq \<rho> p s i", clarsimp)
+  apply(rename_tac p' t tk)
+  apply(rule conjI, clarsimp)
+  apply(frule_tac s=t in available_pos_pstep)
+   apply clarify
+   apply(rename_tac q t')
+   apply(rule_tac a="(p'\<lbrakk>q\<rbrakk>\<^bsub>xs\<^esub>, t')" in someI2)
+    apply assumption
+   apply(clarsimp simp: stepR_def)
+   apply(rule_tac x=True in exI, simp)
+  apply(clarsimp simp: stepR_def)
+  apply(rule_tac x=False in exI, simp)
+  done
+
+ 
+
+lemma locally_seq_jumpfree_fair_ex : 
+"locally_seq p \<Longrightarrow> jumpfree p \<Longrightarrow> fair_ret \<rho> \<Longrightarrow>
+ \<forall>\<sigma>. \<exists>sq\<in>fair_iCOMP \<rho> \<inter> EnvCond_i \<rho> Id. confOf(sq 0) = (p, \<sigma>) "
+  apply(rule allI)
+  apply(rule_tac x="fair_seq \<rho> p \<sigma>" in bexI, simp+)
+  apply(rule conjI, clarsimp simp: fair_iCOMP_def)
+   apply(rule conjI)
+    apply(rule fair_seq_iCOMP)
+   apply clarsimp
+   apply(case_tac "fair_seq \<rho> p \<sigma> i", clarsimp)
+   apply(rename_tac q s tk)
+   apply(subgoal_tac "locally_seq q \<and> jumpfree q")
+    apply(frule_tac s=s in available_pos_pstep)
+    apply clarify
+    apply(subgoal_tac "(SOME x. \<rho> \<turnstile> (q, s) -p\<rightarrow> x) = (q\<lbrakk>p'\<rbrakk>\<^bsub>xs\<^esub>, t)")
+     apply(rule_tac x=i in exI, clarsimp)
+     apply(rule conjI, clarsimp)
+      apply(rule fpos_of_eq, assumption+)
+        apply(erule available_rpos)
+       apply assumption+
+      apply(rule refl)
+     apply clarsimp
+    apply(rule_tac a="(q\<lbrakk>p'\<rbrakk>\<^bsub>xs\<^esub>, t)" in someI2, assumption)
+    apply clarsimp
+    apply(drule locally_seq_jumpfree_pstep_unq, assumption, assumption, assumption)
+    apply simp
+   apply(insert iCOMP_jumpfree[OF fair_seq_iCOMP[where p=p and \<rho>=\<rho>], where j=0, simplified])
+   apply(drule_tac x=\<sigma> in meta_spec, clarsimp)
+   apply(drule_tac x=i in spec, clarsimp)
+   apply(insert iCOMP_jumpfree_locally_seq[OF fair_seq_iCOMP[where p=p and \<rho>=\<rho>], where j=0, simplified])
+   apply(drule_tac x=\<sigma> in meta_spec, clarsimp)
+   apply(drule_tac x=i in spec, clarsimp)
+  apply(clarsimp simp: EnvCond_i_def)
+  apply(rule conjI, rule fair_seq_iCOMP)
+  apply(clarsimp simp: cstep_cond_def)
+  apply(case_tac i, simp+)
+  apply(rename_tac n)
+  apply(case_tac "fair_seq \<rho> p \<sigma> n", clarsimp split: if_splits)
+  done
+
+
+
+end
+
+
